---

title: 
author: 
date: 
geometry: margin=2.5cm
output: 


\usepackage{amsmath}
---
 **Authors: Wojciech Pta≈õ (7042843), Mhd Jawad Al Rahwanji (703890)**



# 2.


## 2.1

The probability of $j$th observation being the first bootstrap observation is equal to $\frac{1}{n}$ because of the uniform distribution. The probability of a complementary event is then equal to $1-\frac{1}{n}$

## 2.2

The probability of $j$th observation being in the bootstrap sample $k$ times can be obtained with binomial distribution:

$P=\binom{n}{k}p^k(1-p)^{n-k}$

In this case $k=0$ and $p=\frac{1}{n}$ because of the normal distribution, so the probability equation changes to:

$P=\frac{n!}{0!*n!}(\frac{1}{n})^0(1-\frac{1}{n})^n=$  
$=(1-\frac{1}{n})^n$ 

Which concudes the proof.

## 2.3

As the value of $n$ increases, the probability from 2.1 converges to 1, while the probability obtained in 2.2 converges to $e^{-1}\approx0.368$